committing just to have a record of this absolute mess

Computability/test.lean
@@ -4,6 +4,219 @@ import Computability.Constructions
 #eval Encodable.encode (Option.some 1:Option ℕ)
 #eval Encodable.encode (Option.some 2:Option ℕ)
 
+
+
+
+
+
+
+
+
+
+
+
+
+
+
+
+
+
+
+section div
+namespace Nat.RecursiveIn.Code
+def c_div_flip2 :=
+  let dividend := succ.comp $ left.comp right
+  let divisor := left
+  let list_of_prev_values := right.comp right
+
+  -- c_l_get_last.comp $
+  c_cov_rec
+
+  (c_const 0) $            -- base case: if dividend is 0, return 0
+
+  c_ifz.comp₂ divisor $    -- in general, test if the divisor is zero
+  pair (c_const 0) $       -- if so, return 0
+  c_if_lt_te.comp₄ dividend divisor (c_const 0) $ -- if dividend < divisor, return 0
+  (succ.comp (c_l_get.comp₂ list_of_prev_values (c_sub.comp₂ dividend divisor))) -- else return (dividend-divisor)/divisor+1
+
+-- def c_div := c_div_flip.comp (pair right left)
+-- i want the inductive case to be simplified to an expression involving c_div_flip2.
+-- this cannot be done after unfolding c_div_flip2, as that will destroy all 'c_div_flip2' 's.
+-- not sure how to do it automatically. in the meanwhile, i can explicitly define it, like below:
+
+-- set_option trace.Meta.Tactic.simp true in
+theorem c_div_flip_evp_aux_aux_test2 :
+  Nat.list_get_last (eval_prim O c_div_flip2 (Nat.pair (d+1) (n+1)))
+    =
+  if n<d then 0 else Nat.list_get_last (eval_prim O c_div_flip2 (Nat.pair (d+1) (n-d))) + 1
+    := by
+
+    rw (config := {occs := .pos [1]}) [c_div_flip2]
+    -- simp? [eval_prim]
+
+    -- simp [eval_prim,
+    --   -c_cov_rec_evp_0,
+    --   -c_cov_rec_evp_1,
+    --   -c_cov_rec_evp_2,
+    --   -c_cov_rec_evp_3,
+    --   -c_cov_rec_evp_4,
+    -- ]
+
+    -- simp only [eval_prim]
+    simp only [c_cov_rec_evp_3]
+    -- simp only [c_cov_rec_evp_0]
+    -- simp? [eval_prim]
+
+    have wtf :
+      eval_prim O
+      (let dividend := succ.comp $ left.comp right
+      let divisor := left
+      let list_of_prev_values := right.comp right
+
+      -- c_l_get_last.comp $
+      c_cov_rec
+
+      (c_const 0) $            -- base case: if dividend is 0, return 0
+
+      c_ifz.comp₂ divisor $    -- in general, test if the divisor is zero
+      pair (c_const 0) $       -- if so, return 0
+      c_if_lt_te.comp₄ dividend divisor (c_const 0) $ -- if dividend < divisor, return 0
+      (succ.comp (c_l_get.comp₂ list_of_prev_values (c_sub.comp₂ dividend divisor)))) -- else return (dividend-divisor)/divisor+1)
+      (Nat.pair (d + 1) n)
+    =
+      eval_prim O c_div_flip2 (Nat.pair (d + 1) n)
+      := by exact rfl
+
+    -- have fyhbuioAWEFBHYUIOASRGYBHUIOASRFGBHUIORFSEBYUIOQ : (eval_prim O
+    --       ((c_const 0).c_cov_rec
+    --         (c_ifz.comp₂ left
+    --           ((c_const 0).pair
+    --             (c_if_lt_te.comp₄ (succ.comp (left.comp right)) left (c_const 0)
+    --               (succ.comp (c_l_get.comp₂ (right.comp right) (c_sub.comp₂ (succ.comp (left.comp right)) left)))))))
+    --       (Nat.pair (d + 1) n)) =eval_prim O c_div_flip2 (Nat.pair (d+1) (n)) := by exact rfl
+    -- rw [fyhbuioAWEFBHYUIOASRGYBHUIOASRFGBHUIORFSEBYUIOQ]
+    
+    rw [wtf]
+    simp [eval_prim]
+    have h0: n-d≤n := by exact sub_le n d
+    #check c_cov_rec_evp_2 h0
+    unfold c_div_flip2
+    rw [c_cov_rec_evp_2 h0]
+
+
+
+    
+    -- simp only [comp₂_evp]
+    -- simp only [eval_prim]
+    -- simp only [l]
+    -- simp only [unpair_pair]
+    -- simp only [c_const_evp]
+    -- simp only [comp₄_evp]
+
+    -- -- simp only [comp₂_evp]
+    -- simp only [eval_prim]
+    -- simp only [l]
+    -- simp only [unpair_pair]
+    -- simp only [c_const_evp]
+    -- -- simp only [comp₄_evp]
+
+    
+    -- simp only [r]
+    -- simp only [succ_eq_add_one]
+    -- simp only [c_sub_evp]
+    -- simp only [unpaired]
+    -- simp only [sub_eq]
+    -- simp only [reduceSubDiff]
+    -- simp only [c_l_get_evp]
+    -- simp only [tsub_le_iff_right]
+    -- simp only [le_add_iff_nonneg_right]
+    -- simp only [_root_.zero_le]
+    -- simp only [c_cov_rec_evp_2]
+    -- simp only [c_if_lt_te_evp]
+    -- simp only [add_lt_add_iff_right]
+    -- simp only [c_ifz_evp]
+    -- simp only [Nat.add_eq_zero]
+    -- simp only [one_ne_zero]
+    -- simp only [and_false]
+    -- simp only [↓reduceIte]
+
+
+
+
+    
+    have rwh : (eval_prim O
+          ((c_const 0).c_cov_rec
+            (c_ifz.comp₂ left
+              ((c_const 0).pair
+                (c_if_lt_te.comp₄ (succ.comp (left.comp right)) left (c_const 0)
+                  (succ.comp (c_l_get.comp₂ (right.comp right) (c_sub.comp₂ (succ.comp (left.comp right)) left)))))))
+          (Nat.pair (d + 1) (n - d))).list_get_last = eval_prim O c_div_flip (Nat.pair (d + 1) (n - d)) := by
+            rw [c_div_flip]
+            simp [eval_prim]
+    rw [rwh]
+    -- calc
+
+    -- rw (config := {occs := .pos [1]}) [c_div_flip]
+    -- simp [eval_prim]
+
+
+
+    -- rw [c_div_flip]
+
+    -- simp only [eval_prim]
+    -- simp [c_cov_rec_evp_0]
+    -- simp [eval_prim]
+
+    -- simp? [eval_prim] says simp only [eval_prim, c_cov_rec_evp_0, comp₂_evp, l, unpair_pair, c_const_evp, comp₄_evp, r,
+    --   succ_eq_add_one, c_sub_evp, unpaired, sub_eq, reduceSubDiff, c_l_get_evp, tsub_le_iff_right,
+    --   le_add_iff_nonneg_right, _root_.zero_le, c_cov_rec_evp_2, c_if_lt_te_evp,
+    --   add_lt_add_iff_right, c_ifz_evp, Nat.add_eq_zero, one_ne_zero, and_false, ↓reduceIte,
+    --   c_l_get_last_evp, list_get_last_append]
+
+
+
+
+
+
+
+
+
+
+
+
+
+
+
+
+
+
+
+
+
+
+
+
+
+
+
+
+
+
+
+
+
+
+
+
+
+
+
+
+
+
+
+
+
 section replace_oracle
 namespace Nat.RecursiveIn.Code
 def encodeCode_replace_oracle (o:ℕ) : Code → ℕ
@@ -36,7 +249,7 @@ def c_replace_oracle :=
   let prec_code       := c_add.comp₂ (            c_mul2.comp $ succ.comp $ c_mul2.comp (pair ml mr)) (c_const 5)
   let rfind'_code     := c_add.comp₂ (succ.comp $ c_mul2.comp $ succ.comp $ c_mul2.comp ml          ) (c_const 5)
 
-  c_l_get_last.comp $
+  -- c_l_get_last.comp $
   c_cov_rec
 
   (c_const 0) $
@@ -52,13 +265,17 @@ def c_replace_oracle :=
 
 -- @[simp] theorem c_replace_oracle_ev_pr:code_prim (c_replace_oracle) := by unfold c_replace_oracle; repeat (constructor; try simp)
 
+set_option maxHeartbeats 5000000 in
 -- set_option maxHeartbeats 1000000 in
 -- set_option maxHeartbeats 1000 in
-@[simp] theorem c_replace_oracle_evp_aux_aux (h:n%4=0): eval_prim O (c_replace_oracle) (Nat.pair o ((n+4)+1)) =
+-- set_option trace.Meta.Tactic.simp true in
+@[simp] theorem c_replace_oracle_evp_aux_aux (h:n%4=0):
+Nat.list_get_last (eval_prim O (c_replace_oracle) (Nat.pair o ((n+4)+1)))
+  =
   -- let m:=n.div2.div2
   let m:=(n/2)/2
-  let ml := eval_prim O (c_replace_oracle) (Nat.pair o m.l)
-  let mr := eval_prim O (c_replace_oracle) (Nat.pair o m.r)
+  let ml := Nat.list_get_last (eval_prim O (c_replace_oracle) (Nat.pair o m.l))
+  let mr := Nat.list_get_last (eval_prim O (c_replace_oracle) (Nat.pair o m.r))
 
   2*(2*(Nat.pair (ml) (mr))  )   + 5
   -- if n%4=0 then 2*(2*(Nat.pair (ml) (mr))  )   + 5 else
@@ -69,10 +286,102 @@ def c_replace_oracle :=
 
 
  := by
-  simp only []
+  -- rw [ml]
   rw (config := {occs := .pos [1]}) [c_replace_oracle]
   -- rw [c_replace_oracle]
-  simp only [eval_prim]
+  simp only [c_cov_rec_evp_3]
+
+
+
+
+
+
+
+
+  have wtfman1 :
+  eval_prim O
+    (  let o               := left
+    let input_to_decode := succ.comp (left.comp right)
+    let comp_hist       := right.comp right
+    let n               := c_sub.comp₂ input_to_decode (c_const 5)
+    let m               := c_div2.comp $ c_div2.comp n
+    let ml              := c_l_get.comp₂ comp_hist (left.comp m)
+    let mr              := c_l_get.comp₂ comp_hist (right.comp m)
+    let nMod4           := c_mod.comp₂ n (c_const 4)
+    let pair_code       := c_add.comp₂ (            c_mul2.comp $             c_mul2.comp (pair ml mr)) (c_const 5)
+    let comp_code       := c_add.comp₂ (succ.comp $ c_mul2.comp $             c_mul2.comp (pair ml mr)) (c_const 5)
+    let prec_code       := c_add.comp₂ (            c_mul2.comp $ succ.comp $ c_mul2.comp (pair ml mr)) (c_const 5)
+    let rfind'_code     := c_add.comp₂ (succ.comp $ c_mul2.comp $ succ.comp $ c_mul2.comp ml          ) (c_const 5)
+
+    -- c_l_get_last.comp $
+    c_cov_rec
+
+    (c_const 0) $
+
+    c_if_eq_te.comp₄ input_to_decode (c_const 1) (c_const 1) $
+    c_if_eq_te.comp₄ input_to_decode (c_const 2) (c_const 2) $
+    c_if_eq_te.comp₄ input_to_decode (c_const 3) (c_const 3) $
+    c_if_eq_te.comp₄ input_to_decode (c_const 4) o           $
+    c_if_eq_te.comp₄ nMod4           (c_const 0) (pair_code) $
+    c_if_eq_te.comp₄ nMod4           (c_const 1) (comp_code) $
+    c_if_eq_te.comp₄ nMod4           (c_const 2) (prec_code) $
+                                                  rfind'_code)
+    (Nat.pair o (n+4))
+  =
+    eval_prim O c_replace_oracle (Nat.pair o (n+4))
+    :=
+  by exact rfl
+  rw [wtfman1]
+
+  simp [eval_prim, h]
+
+  have h2: (n/2/2)≤n := by
+    exact le_trans (Nat.div_le_self _ _) (Nat.div_le_self _ _)
+  -- have h0: (n/2/2).l≤n/2/2 := by
+  --   exact 
+  -- have h1 : (n/2/2).l≤n := by exact 
+  -- have h1 : (n/2/2).l≤n := by exact Nat.le_trans h0 h2
+  -- have h1' : (unpair (n / 2 / 2)).1≤n := by exact Nat.le_trans h0 h2
+  have h3 : (n/2/2).l≤n+4 := by exact le_add_right_of_le (Nat.le_trans (unpair_left_le (n/2/2)) (le_trans (Nat.div_le_self _ _) (Nat.div_le_self _ _)))
+  have h4 : (n/2/2).r≤n+4 := by exact le_add_right_of_le (Nat.le_trans (unpair_right_le (n/2/2)) (le_trans (Nat.div_le_self _ _) (Nat.div_le_self _ _)))
+    
+  -- #check c_cov_rec_evp_2 h1
+  unfold c_replace_oracle
+  rw [c_cov_rec_evp_2 h3]
+  rw [c_cov_rec_evp_2 h4]
+
+  -- simp
+  simp only []
+  simp
+
+  #check mul_comm
+  rw [mul_comm]
+  simp
+  rw [mul_comm]
+  -- exact rfl
+  -- exact rfl
+  
+
+
+
+
+
+
+
+
+
+
+
+
+
+
+
+
+
+
+
+  
+  -- simp only [eval_prim]
 
   -- rw [eval_prim]
   -- simp only [c_cov_rec_evp_0]
